examples/dynamic_isolation/Multicore.v
@@ -95,16 +95,16 @@ Module MachineSemantics (External: External_sig) (EnclaveParams: EnclaveParamete
   Definition get_rf (core: ind_core_id) (st: state) : env_t ContextEnv Rf.R :=
     let koika_st := koika_state st in
     match core with
-    | CoreId0 => ContextEnv.(create) (fun r => ContextEnv.(getenv) koika_st (Machine_Common.core0_rf r))
-    | CoreId1 => ContextEnv.(create) (fun r => ContextEnv.(getenv) koika_st (Machine_Common.core1_rf r))
+    | CoreId0 => ContextEnv.(create) (fun r => ContextEnv.(getenv) koika_st (System.core0_rf r))
+    | CoreId1 => ContextEnv.(create) (fun r => ContextEnv.(getenv) koika_st (System.core1_rf r))
     end.
 
   Definition update_non_koika_st: state -> Log R ContextEnv -> Log R ContextEnv * non_koika_state_t :=
     fun st log =>
       let (mem_log', ext_st') :=
-          Memory.non_koika_update_function ((proj_env Machine_Common.Lift_mem (koika_state st)), non_koika_state st)
-                                           (proj_log Machine_Common.Lift_mem log) in
-      (lift_log Machine_Common.Lift_mem mem_log', ext_st').
+          Memory.non_koika_update_function ((proj_env System.Lift_mem (koika_state st)), non_koika_state st)
+                                           (proj_log System.Lift_mem log) in
+      (lift_log System.Lift_mem mem_log', ext_st').
 
   Definition update_koika (st: koika_state_t) : Log R ContextEnv :=
     interp_scheduler st System.sigma System.rules System.schedule.
@@ -124,19 +124,19 @@ Module MachineSemantics (External: External_sig) (EnclaveParams: EnclaveParamete
     let enclave_data := enclave_config_to_enclave_data config in
     let initial (reg: System.reg_t) :=
         match reg return R reg with
-        | Machine_Common.SM_internal (SM_Common.clk) => clk
-        | Machine_Common.SM_internal SM_Common.enc_data0 =>
+        | System.SM_internal (SM_Common.clk) => clk
+        | System.SM_internal SM_Common.enc_data0 =>
             match core_id with
             | CoreId0 => enclave_data
-            | CoreId1 => System.r (Machine_Common.SM_internal SM_Common.enc_data0)
+            | CoreId1 => System.r (System.SM_internal SM_Common.enc_data0)
             end
-        | Machine_Common.SM_internal SM_Common.enc_data1 =>
+        | System.SM_internal SM_Common.enc_data1 =>
             match core_id with
-            | CoreId0 => System.r (Machine_Common.SM_internal SM_Common.enc_data1)
+            | CoreId0 => System.r (System.SM_internal SM_Common.enc_data1)
             | CoreId1 => enclave_data
             end
-        | Machine_Common.core0_rf s => ContextEnv.(getenv) rf s
-        | Machine_Common.core1_rf s => ContextEnv.(getenv) rf s
+        | System.core0_rf s => ContextEnv.(getenv) rf s
+        | System.core1_rf s => ContextEnv.(getenv) rf s
         | s => System.r s
         end in
     {| koika_state := create ContextEnv System.r;
@@ -151,14 +151,14 @@ Module MachineSemantics (External: External_sig) (EnclaveParams: EnclaveParamete
     let koika_st' :=
       ContextEnv.(create) (fun reg =>
                              match reg return R reg with
-                             | Machine_Common.SM_internal SM_Common.enc_data0 =>
+                             | System.SM_internal SM_Common.enc_data0 =>
                                  match core_id with
                                  | CoreId0 => enclave_data
-                                 | CoreId1 => ContextEnv.(getenv) state (Machine_Common.SM_internal SM_Common.enc_data0)
+                                 | CoreId1 => ContextEnv.(getenv) state (System.SM_internal SM_Common.enc_data0)
                                  end
-                             | Machine_Common.SM_internal SM_Common.enc_data1 =>
+                             | System.SM_internal SM_Common.enc_data1 =>
                                  match core_id with
-                                 | CoreId0 => ContextEnv.(getenv) state (Machine_Common.SM_internal SM_Common.enc_data1)
+                                 | CoreId0 => ContextEnv.(getenv) state (System.SM_internal SM_Common.enc_data1)
                                  | CoreId1 => enclave_data
                                  end
                              | s => ContextEnv.(getenv) state s
@@ -171,13 +171,13 @@ Module MachineSemantics (External: External_sig) (EnclaveParams: EnclaveParamete
   Section Observations.
     (* TODO: turns of duplication *)
     Definition observe_imem_reqs0 (log: Log R ContextEnv) : option (struct_t mem_req) :=
-      (observe_enq0 (Machine_Common.Core0ToSM_IMem MemReq.valid0) eq_refl
-                    (Machine_Common.Core0ToSM_IMem MemReq.data0) eq_refl
+      (observe_enq0 (System.Core0ToSM_IMem MemReq.valid0) eq_refl
+                    (System.Core0ToSM_IMem MemReq.data0) eq_refl
                     log).
 
     Definition observe_imem_reqs1 (log: Log R ContextEnv) : option (struct_t mem_req) :=
-      (observe_enq0 (Machine_Common.Core1ToSM_IMem MemReq.valid0) eq_refl
-                    (Machine_Common.Core1ToSM_IMem MemReq.data0) eq_refl
+      (observe_enq0 (System.Core1ToSM_IMem MemReq.valid0) eq_refl
+                    (System.Core1ToSM_IMem MemReq.data0) eq_refl
                     log).
 
     Definition observe_imem_reqs (log: Log R ContextEnv) (core_id: ind_core_id) : option (struct_t mem_req) :=
@@ -187,12 +187,12 @@ Module MachineSemantics (External: External_sig) (EnclaveParams: EnclaveParamete
       end.
 
     Definition observe_dmem_reqs0 (log: Log R ContextEnv) : option (struct_t mem_req) :=
-      (observe_enq0 (Machine_Common.Core0ToSM_DMem MemReq.valid0) eq_refl
-                    (Machine_Common.Core0ToSM_DMem MemReq.data0) eq_refl
+      (observe_enq0 (System.Core0ToSM_DMem MemReq.valid0) eq_refl
+                    (System.Core0ToSM_DMem MemReq.data0) eq_refl
                     log).
     Definition observe_dmem_reqs1 (log: Log R ContextEnv) : option (struct_t mem_req) :=
-      (observe_enq0 (Machine_Common.Core1ToSM_DMem MemReq.valid0) eq_refl
-                    (Machine_Common.Core1ToSM_DMem MemReq.data0) eq_refl
+      (observe_enq0 (System.Core1ToSM_DMem MemReq.valid0) eq_refl
+                    (System.Core1ToSM_DMem MemReq.data0) eq_refl
                     log).
 
 
@@ -208,13 +208,13 @@ Module MachineSemantics (External: External_sig) (EnclaveParams: EnclaveParamete
       |}.
 
     Definition observe_imem_resps0 (log: Log R ContextEnv) : option (struct_t mem_resp) :=
-      observe_enq1 (Machine_Common.SMToCore0_IMem MemResp.valid0) eq_refl
-                   (Machine_Common.SMToCore0_IMem MemResp.data0) eq_refl
+      observe_enq1 (System.SMToCore0_IMem MemResp.valid0) eq_refl
+                   (System.SMToCore0_IMem MemResp.data0) eq_refl
                    log.
 
     Definition observe_imem_resps1 (log: Log R ContextEnv) : option (struct_t mem_resp) :=
-      observe_enq1 (Machine_Common.SMToCore1_IMem MemResp.valid0) eq_refl
-                   (Machine_Common.SMToCore1_IMem MemResp.data0) eq_refl
+      observe_enq1 (System.SMToCore1_IMem MemResp.valid0) eq_refl
+                   (System.SMToCore1_IMem MemResp.data0) eq_refl
                    log.
 
     Definition observe_imem_resps (log: Log R ContextEnv) (core_id: ind_core_id) : option (struct_t mem_resp) :=
@@ -224,13 +224,13 @@ Module MachineSemantics (External: External_sig) (EnclaveParams: EnclaveParamete
       end.
 
     Definition observe_dmem_resps0 (log: Log R ContextEnv) : option (struct_t mem_resp) :=
-      observe_enq1 (Machine_Common.SMToCore0_DMem MemResp.valid0) eq_refl
-                   (Machine_Common.SMToCore0_DMem MemResp.data0) eq_refl
+      observe_enq1 (System.SMToCore0_DMem MemResp.valid0) eq_refl
+                   (System.SMToCore0_DMem MemResp.data0) eq_refl
                    log.
 
     Definition observe_dmem_resps1 (log: Log R ContextEnv) : option (struct_t mem_resp) :=
-      observe_enq1 (Machine_Common.SMToCore1_DMem MemResp.valid0) eq_refl
-                   (Machine_Common.SMToCore1_DMem MemResp.data0) eq_refl
+      observe_enq1 (System.SMToCore1_DMem MemResp.valid0) eq_refl
+                   (System.SMToCore1_DMem MemResp.data0) eq_refl
                    log.
 
     Definition observe_dmem_resps (log: Log R ContextEnv) (core_id: ind_core_id) : option (struct_t mem_resp) :=
@@ -241,13 +241,13 @@ Module MachineSemantics (External: External_sig) (EnclaveParams: EnclaveParamete
 
 
     Definition observe_enclave_reqs0 (log: Log R ContextEnv) : option (struct_t enclave_req) :=
-      observe_enq0 (Machine_Common.Core0ToSM_Enc EnclaveReq.valid0) eq_refl
-                   (Machine_Common.Core0ToSM_Enc EnclaveReq.data0) eq_refl
+      observe_enq0 (System.Core0ToSM_Enc EnclaveReq.valid0) eq_refl
+                   (System.Core0ToSM_Enc EnclaveReq.data0) eq_refl
                    log.
 
     Definition observe_enclave_reqs1 (log: Log R ContextEnv) : option (struct_t enclave_req) :=
-      observe_enq0 (Machine_Common.Core1ToSM_Enc EnclaveReq.valid0) eq_refl
-                   (Machine_Common.Core1ToSM_Enc EnclaveReq.data0) eq_refl
+      observe_enq0 (System.Core1ToSM_Enc EnclaveReq.valid0) eq_refl
+                   (System.Core1ToSM_Enc EnclaveReq.data0) eq_refl
                    log.
 
     Definition observe_enclave_reqs (log: Log R ContextEnv) (core_id: ind_core_id) : option (struct_t enclave_req) :=
@@ -261,13 +261,13 @@ Module MachineSemantics (External: External_sig) (EnclaveParams: EnclaveParamete
 
     (* TODO (slight hack): If write reg_proc_reset == Restart, treat as switching enclaves *)
     Definition observe_enclave_enter0 (log: Log R ContextEnv) : bool :=
-      match latest_write log Machine_Common.purge_core0 with
+      match latest_write log System.purge_core0 with
       | Some v => bits_eqb v ENUM_purge_restart
       | None => false
       end.
 
     Definition observe_enclave_enter1 (log: Log R ContextEnv) : bool :=
-      match latest_write log Machine_Common.purge_core1 with
+      match latest_write log System.purge_core1 with
       | Some v => bits_eqb v ENUM_purge_restart
       | None => false
       end.
@@ -279,7 +279,7 @@ Module MachineSemantics (External: External_sig) (EnclaveParams: EnclaveParamete
       end.
 
     Definition observe_enclave_exit0 (log: Log R ContextEnv) : bool :=
-      match latest_write log (Machine_Common.SM_internal SM_Common.enc_data0) with
+      match latest_write log (System.SM_internal SM_Common.enc_data0) with
       | Some v =>
           let data := EnclaveInterface.extract_enclave_data v in
           bits_eqb (EnclaveInterface.enclave_data_valid data) Ob~0
@@ -287,7 +287,7 @@ Module MachineSemantics (External: External_sig) (EnclaveParams: EnclaveParamete
       end.
 
     Definition observe_enclave_exit1 (log: Log R ContextEnv) : bool :=
-      match latest_write log (Machine_Common.SM_internal SM_Common.enc_data1) with
+      match latest_write log (System.SM_internal SM_Common.enc_data1) with
       | Some v =>
           let data := EnclaveInterface.extract_enclave_data v in
           bits_eqb (EnclaveInterface.enclave_data_valid data) Ob~0
